[lf] wip.

aneris/examples/reliable_communication/lib/repdb/proof/leader/clients_mt_user_params.v
@@ -18,7 +18,6 @@ From aneris.examples.reliable_communication.lib.repdb.resources
 From aneris.examples.reliable_communication.lib.repdb.proof
      Require Import log_proof repdb_serialization.
 
-
 Import gen_heap_light.
 Import lock_proof.
 
@@ -84,84 +83,3 @@ Section MT_user_params.
     |}.
 
 End MT_user_params.
-
-Section MT_spec_params.
-
-  Context `{!anerisG Mdl Σ, !DB_params, !IDBG Σ}.
-  Context (γL γM mγ : gname).
-  Context (mv : val).
-  Context (kvsL logL : loc).
-
-  Definition handler_cloj : val :=
-    λ: "mv" "reqv", client_request_handler_at_leader #kvsL #logL "mv" "reqv".
-
-  Notation MTU := (client_handler_at_leader_user_params γL γM).
-
-  Lemma client_request_handler_at_leader_spec  :
-    ∀ reqv reqd,
-    {{{ is_monitor MTU.(MTS_mN) (ip_of_address MTU.(MTS_saddr)) mγ mv
-               (leader_local_main_inv_def γL kvsL logL) ∗
-           lock_proof.locked mγ ∗ (leader_local_main_inv_def γL kvsL logL) ∗
-           MTU.(MTS_handler_pre) reqv reqd }}}
-       handler_cloj mv reqv @[ip_of_address MTU.(MTS_saddr)]
-    {{{ repv repd, RET repv;
-        ⌜Serializable (rep_l2c_serialization) repv⌝ ∗
-        lock_proof.locked mγ ∗ (leader_local_main_inv_def γL kvsL logL) ∗
-        MTU.(MTS_handler_post) repv reqd repd }}}.
-  Proof.
-  Admitted.
-   (* iIntros (Φ) "(#Hmon & Hkey & HR & Hpre) HΦ".
-    rewrite /client_request_handler_at_leader.
-    wp_pures.
-    rewrite /ReqPre.
-    iDestruct "Hpre" as "(#HGinv & [HpreW | HpreR])".
-    - admit.
-    - iDestruct "HpreR" as (k we q Hkeys Hreqd ->) "Hk".
-      wp_pures.
-      rewrite{2} /leader_local_main_inv_def.
-      iDestruct "HR" as (lV mV mM lM Hmap Hlog HvalidL) "(Hm & Hl & HlogL)".
-      wp_load.
-      wp_apply (wp_map_lookup $! Hmap).
-      iIntros (v Hv).
-      wp_pures.
-      destruct (mM !! k) eqn:Hmk; rewrite Hmk in Hv.
-      + admit.
-      + iApply ("HΦ" $! _ (inr None)).
-        iSplit.
-        * rewrite Hv. rewrite /rep_l2c_serialization.
-          iPureIntro.
-          rewrite /Serializable /= /sum_valid_val /=; eauto.
-          exists (InjLV #()). right. split; first done. by right.
-        * iFrame "Hkey".
-          iSplitR "Hk".
-          ** admit.
-          ** iRight. iIntros (k0 wo0 q0 Hreqd0).
-             iExists v.
-             iSplit.
-             admit.
-             iSplit; first done.
-             rewrite Hreqd0 in Hreqd. inversion Hreqd. subst.
-             iFrame. iLeft. admit.
-
-          rewrite /option_valid_val.
-          exists (InjLV #()).
-          Eapply option_is_ser_valid. rewrite option_valid_val. /=; eauto..
-          eauto. done. apply (sum_is_ser_valid _ _ _ ""). simplify_eq.
-          simpl. iPureIntro. simplify_eq /=.
-          eapply sum_is_ser_valid. rewrite /sum_is_ser. simplify_eq /=.
-          eexists _, _. right. split; eauto. done.
-       + admit.
-      + iFrame "Hkey". *)
-
-
-  Global Instance client_handler_at_leader_spec_params :
-    @MTS_spec_params _ _ _ _ MTU :=
-    {|
-      MTS_mR := (leader_local_main_inv_def γL kvsL logL);
-      MTS_mγ := mγ;
-      MTS_mv := mv;
-      MTS_handler := handler_cloj;
-      MTS_handler_spec := client_request_handler_at_leader_spec;
-    |}.
-
-End MT_spec_params.
