aneris/examples/reliable_communication/lib/repdb/proof/leader/proof_of_client_handler.v
@@ -1,0 +1,104 @@
+From iris.algebra Require Import agree auth excl gmap dfrac.
+From iris.algebra.lib Require Import mono_list.
+From iris.base_logic Require Import invariants.
+From iris.bi.lib Require Import fractional.
+From iris.proofmode Require Import tactics coq_tactics reduction spec_patterns.
+From aneris.lib Require Import gen_heap_light.
+From aneris.aneris_lang Require Import lang resources inject tactics proofmode.
+From aneris.aneris_lang.lib Require Import list_proof monitor_proof lock_proof map_proof.
+From aneris.aneris_lang.lib.serialization Require Import serialization_proof.
+From aneris.aneris_lang.program_logic Require Import aneris_lifting.
+From aneris.aneris_lang.program_logic Require Import aneris_weakestpre.
+From aneris.examples.reliable_communication.prelude Require Import ser_inj.
+From aneris.examples.reliable_communication.lib.mt_server Require Import user_params.
+From aneris.examples.reliable_communication.lib.repdb Require Import repdb_code model.
+From aneris.examples.reliable_communication.lib.repdb.spec Require Import db_params events.
+From aneris.examples.reliable_communication.lib.repdb.resources
+     Require Import ras resources_def resources_global_inv resources_local_inv.
+From aneris.examples.reliable_communication.lib.repdb.proof
+     Require Import log_proof repdb_serialization.
+From aneris.examples.reliable_communication.lib.repdb.proof.leader
+     Require Import clients_mt_user_params.
+
+Import gen_heap_light.
+Import lock_proof.
+
+Section Clients_MT_spec_params.
+
+  Context `{!anerisG Mdl Σ, !DB_params, !IDBG Σ}.
+  Context (γL γM : gname).
+  Context (mγ : gname) (mv : val) (kvsL logL : loc).
+
+  Definition handler_cloj : val :=
+    λ: "mv" "reqv", client_request_handler_at_leader #kvsL #logL "mv" "reqv".
+
+  Notation MTU := (client_handler_at_leader_user_params γL γM).
+
+  Lemma client_request_handler_at_leader_spec  :
+    ∀ reqv reqd,
+    {{{ is_monitor MTU.(MTS_mN) (ip_of_address MTU.(MTS_saddr)) mγ mv
+               (leader_local_main_inv_def γL kvsL logL) ∗
+           lock_proof.locked mγ ∗ (leader_local_main_inv_def γL kvsL logL) ∗
+           MTU.(MTS_handler_pre) reqv reqd }}}
+       handler_cloj mv reqv @[ip_of_address MTU.(MTS_saddr)]
+    {{{ repv repd, RET repv;
+        ⌜Serializable (rep_l2c_serialization) repv⌝ ∗
+        lock_proof.locked mγ ∗ (leader_local_main_inv_def γL kvsL logL) ∗
+        MTU.(MTS_handler_post) repv reqd repd }}}.
+  Proof.
+  Admitted.
+   (* iIntros (Φ) "(#Hmon & Hkey & HR & Hpre) HΦ".
+    rewrite /client_request_handler_at_leader.
+    wp_pures.
+    rewrite /ReqPre.
+    iDestruct "Hpre" as "(#HGinv & [HpreW | HpreR])".
+    - admit.
+    - iDestruct "HpreR" as (k we q Hkeys Hreqd ->) "Hk".
+      wp_pures.
+      rewrite{2} /leader_local_main_inv_def.
+      iDestruct "HR" as (lV mV mM lM Hmap Hlog HvalidL) "(Hm & Hl & HlogL)".
+      wp_load.
+      wp_apply (wp_map_lookup $! Hmap).
+      iIntros (v Hv).
+      wp_pures.
+      destruct (mM !! k) eqn:Hmk; rewrite Hmk in Hv.
+      + admit.
+      + iApply ("HΦ" $! _ (inr None)).
+        iSplit.
+        * rewrite Hv. rewrite /rep_l2c_serialization.
+          iPureIntro.
+          rewrite /Serializable /= /sum_valid_val /=; eauto.
+          exists (InjLV #()). right. split; first done. by right.
+        * iFrame "Hkey".
+          iSplitR "Hk".
+          ** admit.
+          ** iRight. iIntros (k0 wo0 q0 Hreqd0).
+             iExists v.
+             iSplit.
+             admit.
+             iSplit; first done.
+             rewrite Hreqd0 in Hreqd. inversion Hreqd. subst.
+             iFrame. iLeft. admit.
+
+          rewrite /option_valid_val.
+          exists (InjLV #()).
+          Eapply option_is_ser_valid. rewrite option_valid_val. /=; eauto..
+          eauto. done. apply (sum_is_ser_valid _ _ _ ""). simplify_eq.
+          simpl. iPureIntro. simplify_eq /=.
+          eapply sum_is_ser_valid. rewrite /sum_is_ser. simplify_eq /=.
+          eexists _, _. right. split; eauto. done.
+       + admit.
+      + iFrame "Hkey". *)
+
+
+  Global Instance client_handler_at_leader_spec_params :
+    @MTS_spec_params _ _ _ _ MTU :=
+    {|
+      MTS_mR := (leader_local_main_inv_def γL kvsL logL);
+      MTS_mγ := mγ;
+      MTS_mv := mv;
+      MTS_handler := handler_cloj;
+      MTS_handler_spec := client_request_handler_at_leader_spec;
+    |}.
+
+End Clients_MT_spec_params.
